add proof of shuffle_core_spec lemma

code/hash/Hacl.Spec.SHA2.Equiv.fst
@@ -15,33 +15,116 @@ module LSeq = Lib.Sequence
 
 #set-options "--z3rlimit 50 --max_fuel 0 --max_ifuel 0"
 
-let _Ch_lemma #a #m x y z :
-  Lemma (vec_v (_Ch #a #m x y z) ==
-    LSeq.createi (lanes a m) (fun i -> Spec._Ch a (vec_v x).[i] (vec_v y).[i] (vec_v z).[i]))
- =
-  LSeq.eq_intro (vec_v (_Ch #a #m x y z))
-    (LSeq.createi (lanes a m) (fun i -> Spec._Ch a (vec_v x).[i] (vec_v y).[i] (vec_v z).[i]))
+val _Ch_lemma: #a:sha2_alg -> #m:m_spec -> x:element_t a m -> y:element_t a m -> z:element_t a m ->
+  Lemma (forall (l:nat{l < lanes a m}).{:pattern (vec_v (_Ch x y z)).[l]}
+    (vec_v (_Ch #a #m x y z)).[l] == Spec._Ch a (vec_v x).[l] (vec_v y).[l] (vec_v z).[l])
+  [SMTPat (_Ch x y z)]
+
+let _Ch_lemma #a #m x y z = ()
 
 
-let _Maj_lemma #a #m x y z :
-  Lemma (vec_v (_Maj #a #m x y z) ==
-    LSeq.createi (lanes a m) (fun i -> Spec._Maj a (vec_v x).[i] (vec_v y).[i] (vec_v z).[i]))
- =
-  LSeq.eq_intro (vec_v (_Maj #a #m x y z))
-    (LSeq.createi (lanes a m) (fun i -> Spec._Maj a (vec_v x).[i] (vec_v y).[i] (vec_v z).[i]))
+val _Maj_lemma: #a:sha2_alg -> #m:m_spec -> x:element_t a m -> y:element_t a m -> z:element_t a m ->
+  Lemma (forall (l:nat{l < lanes a m}).{:pattern (vec_v (_Maj x y z)).[l]}
+    (vec_v (_Maj #a #m x y z)).[l] == Spec._Maj a (vec_v x).[l] (vec_v y).[l] (vec_v z).[l])
+  [SMTPat (_Maj x y z)]
+
+let _Maj_lemma #a #m x y z = ()
 
 
-let _Sigma0_lemma #a #m x : Lemma (vec_v (_Sigma0 #a #m x) == LSeq.map (Spec._Sigma0 a) (vec_v x)) =
-  LSeq.eq_intro (vec_v (_Sigma0 #a #m x)) (LSeq.map (Spec._Sigma0 a) (vec_v x))
+val _Sigma0_lemma: #a:sha2_alg -> #m:m_spec -> x:element_t a m ->
+  Lemma (forall (l:nat{l < lanes a m}).{:pattern (vec_v (_Sigma0 x)).[l]}
+    (vec_v (_Sigma0 #a #m x)).[l] == Spec._Sigma0 a (vec_v x).[l])
+  [SMTPat (_Sigma0 x)]
 
-let _Sigma1_lemma #a #m x : Lemma (vec_v (_Sigma1 #a #m x) == LSeq.map (Spec._Sigma1 a) (vec_v x)) =
-  LSeq.eq_intro (vec_v (_Sigma1 #a #m x)) (LSeq.map (Spec._Sigma1 a) (vec_v x))
+let _Sigma0_lemma #a #m x = ()
 
-let _sigma0_lemma #a #m x : Lemma (vec_v (_sigma0 #a #m x) == LSeq.map (Spec._sigma0 a) (vec_v x)) =
-  LSeq.eq_intro (vec_v (_sigma0 #a #m x)) (LSeq.map (Spec._sigma0 a) (vec_v x))
 
-let _sigma1_lemma #a #m x : Lemma (vec_v (_sigma1 #a #m x) == LSeq.map (Spec._sigma1 a) (vec_v x)) =
-  LSeq.eq_intro (vec_v (_sigma1 #a #m x)) (LSeq.map (Spec._sigma1 a) (vec_v x))
+val _Sigma1_lemma: #a:sha2_alg -> #m:m_spec -> x:element_t a m ->
+  Lemma (forall (l:nat{l < lanes a m}).{:pattern (vec_v (_Sigma1 x)).[l]}
+    (vec_v (_Sigma1 #a #m x)).[l] == Spec._Sigma1 a (vec_v x).[l])
+  [SMTPat (_Sigma1 x)]
+
+let _Sigma1_lemma #a #m x = ()
+
+
+val _sigma0_lemma: #a:sha2_alg -> #m:m_spec -> x:element_t a m ->
+  Lemma (forall (l:nat{l < lanes a m}).{:pattern (vec_v (_sigma0 x)).[l]}
+    (vec_v (_sigma0 #a #m x)).[l] == Spec._sigma0 a (vec_v x).[l])
+  [SMTPat (_sigma0 x)]
+
+let _sigma0_lemma #a #m x = ()
+
+
+val _sigma1_lemma: #a:sha2_alg -> #m:m_spec -> x:element_t a m ->
+  Lemma (forall (l:nat{l < lanes a m}).{:pattern (vec_v (_sigma1 x)).[l]}
+    (vec_v (_sigma1 #a #m x)).[l] == Spec._sigma1 a (vec_v x).[l])
+  [SMTPat (_sigma1 x)]
+
+let _sigma1_lemma #a #m x = ()
+
+
+val seq_of_list_is_create8: #a:Type -> x0:a -> x1:a -> x2:a -> x3:a -> x4:a -> x5:a -> x6:a -> x7:a ->
+  Lemma (create8 x0 x1 x2 x3 x4 x5 x6 x7 == Seq.seq_of_list [x0; x1; x2; x3; x4; x5; x6; x7])
+
+let seq_of_list_is_create8 #a x0 x1 x2 x3 x4 x5 x6 x7 =
+  let rp = Seq.seq_of_list [x0; x1; x2; x3; x4; x5; x6; x7] in
+  assert_norm (length rp == 8);
+  let lp = create8 x0 x1 x2 x3 x4 x5 x6 x7 in
+
+  let aux (i:nat{i < 8}) : Lemma (Seq.index lp i == Seq.index rp i) =
+    assert_norm (Seq.index lp i == Seq.index rp i) in
+
+  Classical.forall_intro aux;
+  eq_intro rp lp
+
+
+val shuffle_core_pre_create8: a:sha2_alg -> k_t:word a -> ws_t:word a -> hash:words_state a -> words_state a
+let shuffle_core_pre_create8 a k_t ws_t hash =
+  let a0 = Seq.index hash 0 in
+  let b0 = Seq.index hash 1 in
+  let c0 = Seq.index hash 2 in
+  let d0 = Seq.index hash 3 in
+  let e0 = Seq.index hash 4 in
+  let f0 = Seq.index hash 5 in
+  let g0 = Seq.index hash 6 in
+  let h0 = Seq.index hash 7 in
+
+  let t1 = h0 +. (Spec._Sigma1 a e0) +. (Spec._Ch a e0 f0 g0) +. k_t +. ws_t in
+  let t2 = (Spec._Sigma0 a a0) +. (Spec._Maj a a0 b0 c0) in
+  create8 (t1 +. t2) a0 b0 c0 (d0 +. t1) e0 f0 g0
+
+
+val shuffle_core_pre_create8_lemma: a:sha2_alg -> k_t:word a -> ws_t:word a -> hash:words_state a ->
+  Lemma (Spec.shuffle_core_pre a k_t ws_t hash == shuffle_core_pre_create8 a k_t ws_t hash)
+let shuffle_core_pre_create8_lemma a k_t ws_t hash =
+  let a0 = Seq.index hash 0 in
+  let b0 = Seq.index hash 1 in
+  let c0 = Seq.index hash 2 in
+  let d0 = Seq.index hash 3 in
+  let e0 = Seq.index hash 4 in
+  let f0 = Seq.index hash 5 in
+  let g0 = Seq.index hash 6 in
+  let h0 = Seq.index hash 7 in
+
+  let t1 = h0 +. (Spec._Sigma1 a e0) +. (Spec._Ch a e0 f0 g0) +. k_t +. ws_t in
+  let t2 = (Spec._Sigma0 a a0) +. (Spec._Maj a a0 b0 c0) in
+  seq_of_list_is_create8 (t1 +. t2) a0 b0 c0 (d0 +. t1) e0 f0 g0
+
+
+
+noextract
+let state_spec_v_l (#a:sha2_alg) (#m:m_spec) (st:state_spec a m) (l:nat{l < lanes a m}) : words_state a =
+  create8
+    (vec_v st.[0]).[l] (vec_v st.[1]).[l] (vec_v st.[2]).[l] (vec_v st.[3]).[l]
+    (vec_v st.[4]).[l] (vec_v st.[5]).[l] (vec_v st.[6]).[l] (vec_v st.[7]).[l]
+
+noextract
+let ws_spec_v_l (#a:sha2_alg) (#m:m_spec) (st:ws_spec a m) (l:nat{l < lanes a m}) : lseq (word a) 16 =
+  create16
+    (vec_v st.[0]).[l] (vec_v st.[1]).[l] (vec_v st.[2]).[l] (vec_v st.[3]).[l]
+    (vec_v st.[4]).[l] (vec_v st.[5]).[l] (vec_v st.[6]).[l] (vec_v st.[7]).[l]
+    (vec_v st.[8]).[l] (vec_v st.[9]).[l] (vec_v st.[10]).[l] (vec_v st.[11]).[l]
+    (vec_v st.[12]).[l] (vec_v st.[13]).[l] (vec_v st.[14]).[l] (vec_v st.[15]).[l]
 
 
 val shuffle_core_spec_lemma_l:
@@ -52,10 +135,14 @@ val shuffle_core_spec_lemma_l:
   -> st:state_spec a m
   -> l:nat{l < lanes a m} ->
   Lemma
-   ((state_spec_v (shuffle_core_spec k_t ws_t st)).[l] ==
-     Spec.shuffle_core_pre a k_t (vec_v ws_t).[l] (state_spec_v st).[l])
+   (state_spec_v_l (shuffle_core_spec k_t ws_t st) l ==
+    Spec.shuffle_core_pre a k_t (vec_v ws_t).[l] (state_spec_v_l st l))
 
-let shuffle_core_spec_lemma_l #a #m k_t ws_t st l = admit()
+let shuffle_core_spec_lemma_l #a #m k_t ws_t st l =
+  eq_intro #(word a) #(state_word_length a)
+    (state_spec_v_l (shuffle_core_spec k_t ws_t st) l)
+    (shuffle_core_pre_create8 a k_t (vec_v ws_t).[l] (state_spec_v_l st l));
+  shuffle_core_pre_create8_lemma a k_t (vec_v ws_t).[l] (state_spec_v_l st l)
 
 
 val ws_next_inner_lemma_l:
